examples/unit-tests/format.fst
@@ -1,80 +1,57 @@
-module Array 
-(* See examples/sep/array.fst for a full array theory 
-   (still to be ported to new syntax, so including a 
-    subset of its signature here) *)
-
-type seq : Type -> Type
-type Equal : #'a:Type -> seq 'a -> seq 'a -> Type
-assume logic val append : seq 'a -> seq 'a -> Tot (seq 'a)
-assume logic val slice : seq 'a -> int -> int -> Tot (seq 'a)
-assume logic val length : seq 'a -> Tot nat
-assume logic val create : int -> 'a -> Tot (seq 'a)
-
-
 module Format
 open Prims.PURE
 open String
 open Array
 
-type message = seq char//byte
-type msg (l:nat) = m:message{length m == l}
 
-(* lemma *) 
-val append_check: b1:message -> b2:message -> c1:message -> c2:message -> Tot bool (ensures \b -> b==true <==> b1==c1 /\ b2==c2)
+type message = seq char
+type msg (l:nat) = m:message{length m==l}
 
-val append_inj_l: #l:nat 
-               -> b1:msg l -> b2:message 
-               -> c1:msg l -> c2:message{append b1 b2 == append c1 c2} 
-               -> Tot (u:unit{Equal b1 c1 /\ Equal b2 c2})
-let rec append_inj_l l b1 b2 c1 c2 (* {decreases l} *) = match l with
+val append_inj_l: l:nat
+               -> b1:message -> b2:message
+               -> c1:message -> c2:message
+               -> Pure unit
+                       (requires (l==length b1 /\ l==length c1 /\ append b1 b2==append c1 c2))
+                       (ensures \x -> (Equal b1 c1 /\ Equal b2 c2))
+let rec append_inj_l l b1 b2 c1 c2 = match l with
   | 0 -> ()
-     (* assert (Equal b1 c1); *)
-     (* assert (append b1 b2 == b2); *)
-     (* assert (append c1 c2 == c2) *)
+  | _ -> append_inj_l (l - 1) (slice b1 1 l) b2 (slice c1 1 l) c2
 
-  | n ->
-     append_inj_l #(n - 1) (slice b1 1 n) b2 (slice c1 1 n) c2;
-     //b2 == c2
-     //append b1 b2 = append c1 c2
-     //append (slice b1 0 1) (append (slice b1 1 n) b2) ==
-     //append (slice c1 0 1) (append (slice c1 1 n) b2) ==
-     assert (append (slice b1 0 1) (slice b1 1 n) ==
-             append (slice c1 0 1) (slice c1 1 n))
 
-let tag0 = create 1 0uy
-let tag1 = create 1 1uy
+(* let tag0 = create 1 0uy *)
+(* let tag1 = create 1 1uy *)
 
-type UInt16 (i:int) = (b2t (0 <= i) /\ b2t (i < 65536))
-type uint16 = i:int{UInt16 i}
-assume logic val utf8: s:string -> Tot (m:message{length m <= strlen s}) //this spec is accurate for ASCII strings
-assume logic val two:nat
-assume logic val uint16_to_bytes: uint16 -> Tot (msg two)
-type string16 = s:string{UInt16 (length (utf8 s))}
+(* type UInt16 (i:int) = (b2t (0 <= i) /\ b2t (i < 65536)) *)
+(* type uint16 = i:int{UInt16 i} *)
+(* assume logic val utf8: s:string -> Tot (m:message{length m <= strlen s}) //this spec is accurate for ASCII strings *)
+(* assume logic val two:nat *)
+(* assume logic val uint16_to_bytes: uint16 -> Tot (msg two) *)
+(* type string16 = s:string{UInt16 (length (utf8 s))} *)
 
-(* assume UTF8_inj:   forall s0 s1.{:pattern (Equal (utf8 s0) (utf8 s1))} utf8 s0==utf8 s1 ==> s0==s1 *)
-assume UINT16_inj: forall s0 s1. Equal (uint16_to_bytes s0) (uint16_to_bytes s1)
-                             ==> s0==s1
+(* (\* assume UTF8_inj:   forall s0 s1.{:pattern (Equal (utf8 s0) (utf8 s1))} utf8 s0==utf8 s1 ==> s0==s1 *\) *)
+(* assume UINT16_inj: forall s0 s1. Equal (uint16_to_bytes s0) (uint16_to_bytes s1) *)
+(*                              ==> s0==s1 *)
 
-logic val request : string -> Tot message
-let request s = append tag0 (utf8 s)
+(* logic val request : string -> Tot message *)
+(* let request s = append tag0 (utf8 s) *)
 
-logic val response: string16 -> string -> Tot message
-let response s t =
-  let lb = uint16_to_bytes (length (utf8 s)) in
-  append tag1 (append lb 
-                      (append (utf8 s) 
-                              (utf8 t)))
+(* logic val response: string16 -> string -> Tot message *)
+(* let response s t = *)
+(*   let lb = uint16_to_bytes (length (utf8 s)) in *)
+(*   append tag1 (append lb  *)
+(*                       (append (utf8 s)  *)
+(*                               (utf8 t))) *)
 
-(* ask !v,v',s,s',t'. (Requested(v,s) /\ Responded(v',s',t')) -> (v <> v') *)
-(* lemma *) 
-val req_resp_distinct: s:string -> s':string16 -> t':string -> Tot (u:unit{request s =!= response s' t'})
-let req_resp_distinct s s' t' = ()
+(* (\* ask !v,v',s,s',t'. (Requested(v,s) /\ Responded(v',s',t')) -> (v <> v') *\) *)
+(* (\* lemma *\)  *)
+(* val req_resp_distinct: s:string -> s':string16 -> t':string -> Tot (u:unit{request s =!= response s' t'}) *)
+(* let req_resp_distinct s s' t' = () *)
 
-query ReqInj: forall s s'. request s==request s' ==> s==s'
+(* query ReqInj: forall s s'. request s==request s' ==> s==s' *)
 
-(* ask !v,s,s',t,t'. (Responded(v,s,t) /\ Responded(v,s',t')) -> (s = s' /\ t = t') *)
-(* ask !v,v',s,s'. (Requested(v,s) /\ Requested(v',s') /\ v = v') -> (s = s') *)
-(* ask !v,s,s',t,t'. (Responded(v,s,t) /\ Responded(v,s',t')) -> (s = s' /\ t = t') *)
+(* (\* ask !v,s,s',t,t'. (Responded(v,s,t) /\ Responded(v,s',t')) -> (s = s' /\ t = t') *\) *)
+(* (\* ask !v,v',s,s'. (Requested(v,s) /\ Requested(v',s') /\ v = v') -> (s = s') *\) *)
+(* (\* ask !v,s,s',t,t'. (Responded(v,s,t) /\ Responded(v,s',t')) -> (s = s' /\ t = t') *\) *)
      
      
 
